updates

Veritas.Verifier.Merkle.fst
@@ -1358,13 +1358,12 @@ let rec lemma_not_init_equiv_root_reachable (itsl: TL.eac_log) (k:key):
       lemma_not_init_equiv_root_reachable_extend_ptrfn_unchanged itsl k
   )
 
-let rec first_root_reachable_ancestor (itsl: TL.eac_log) (k:key):
-  Tot (k':key{root_reachable itsl k' /\
+let rec first_root_reachable_ancestor (pf:ptrfn) (k:key):
+  Tot (k':key{BP.root_reachable pf k' /\
               is_desc k k'})
   (decreases (depth k)) =
-  let pf = eac_ptrfn itsl in
 
-  if root_reachable itsl k then (
+  if BP.root_reachable pf k then (
     lemma_desc_reflexive k;
     k
   )
@@ -1373,42 +1372,39 @@ let rec first_root_reachable_ancestor (itsl: TL.eac_log) (k:key):
     lemma_reachable_reflexive pf Root;
 
     (* since k is not root_reachable, k cannot be Root *)
-    assert(k <> Root);
+    // assert(k <> Root);
 
     (* so, k has a parent *)
     let kp = parent k in
 
     (* recurse ... *)
-    let k' = first_root_reachable_ancestor itsl kp in
+    let k' = first_root_reachable_ancestor pf kp in
 
     lemma_parent_ancestor k;
     lemma_desc_transitive k kp k';
     k'
   )
 
-(* the ancestor who holds the proof of the value of key k *)
-let proving_ancestor (itsl: TL.eac_log) (k:key{k <> Root}):
-  k':key{is_proper_desc k k'} =
-  let pf = eac_ptrfn itsl in
-  lemma_not_init_equiv_root_reachable itsl k;
-
-  if root_reachable itsl k then
-    //assert(not (is_eac_state_init itsl k));
-    prev_in_path pf k Root
-  else first_root_reachable_ancestor itsl k
-
-let lemma_proving_ancestor_root_reachable (itsl: TL.eac_log) (k:key{k <> Root}):
-  Lemma (let k' = proving_ancestor itsl k in
-         root_reachable itsl k') = ()
-
-let rec lemma_first_root_reachable_ancestor_greatest_depth (itsl: TL.eac_log) (k: key) (k2: key{is_proper_desc k k2}):
-  Lemma (requires (root_reachable itsl k2))
-        (ensures (depth k2 <= depth (first_root_reachable_ancestor itsl k)))
+let rec lemma_feq_first_root_reachable_ancestor (pf1 pf2: ptrfn) (k:key):
+  Lemma (requires (feq_ptrfn pf1 pf2))
+        (ensures (first_root_reachable_ancestor pf1 k = first_root_reachable_ancestor pf2 k)) 
         (decreases (depth k)) = 
-  let krr = first_root_reachable_ancestor itsl k in
+  lemma_reachable_feq pf1 pf2 k Root;        
+  if BP.root_reachable pf1 k then ()
+  else (
+    (* root is reachable from itself *)
+    lemma_reachable_reflexive pf1 Root;   
+    lemma_feq_first_root_reachable_ancestor pf1 pf2 (parent k)
+  )
+
+let rec lemma_first_root_reachable_ancestor_greatest_depth (pf:ptrfn) (k: key) (k2: key{is_proper_desc k k2}):
+  Lemma (requires (BP.root_reachable pf k2))
+        (ensures (depth k2 <= depth (first_root_reachable_ancestor pf k)))
+        (decreases (depth k)) = 
+  let krr = first_root_reachable_ancestor pf k in
   lemma_proper_desc_depth_monotonic k k2;
 
-  if root_reachable itsl k then ()    
+  if BP.root_reachable pf k then ()    
   
   else (
     let kp = parent k in
@@ -1425,9 +1421,33 @@ let rec lemma_first_root_reachable_ancestor_greatest_depth (itsl: TL.eac_log) (k
       else lemma_proper_desc_depth_monotonic k2 kp
     )
     else 
-      lemma_first_root_reachable_ancestor_greatest_depth itsl kp k2
-
+      lemma_first_root_reachable_ancestor_greatest_depth pf kp k2
   )
+
+
+let proving_ancestor_pf (pf: ptrfn) (k: key {k <> Root}):
+  k':key{is_proper_desc k k'} = 
+  if BP.root_reachable pf k then
+    prev_in_path pf k Root
+  else first_root_reachable_ancestor pf k
+
+let lemma_feq_proving_ancestor (pf1: ptrfn) (pf2: ptrfn) (k: key {k <> Root}):
+  Lemma (requires (feq_ptrfn pf1 pf2))
+        (ensures (proving_ancestor_pf pf1 k = proving_ancestor_pf pf2 k)) =
+  lemma_reachable_feq pf1 pf2 k Root;
+  if BP.root_reachable pf1 k then
+    lemma_prev_in_path_feq pf1 pf2 k Root
+  else lemma_feq_first_root_reachable_ancestor pf1 pf2 k
+
+(* the ancestor who holds the proof of the value of key k *)
+let proving_ancestor (itsl: TL.eac_log) (k:key{k <> Root}):
+  k':key{is_proper_desc k k'} =
+  let pf = eac_ptrfn itsl in
+  proving_ancestor_pf pf k
+
+let lemma_proving_ancestor_root_reachable (itsl: TL.eac_log) (k:key{k <> Root}):
+  Lemma (let k' = proving_ancestor itsl k in
+         root_reachable itsl k') = ()
 
 let lemma_proving_ancestor_greatest_depth (itsl: TL.eac_log) (k:key{k <> Root}) (k2: key{is_proper_desc k k2}):
   Lemma (requires (root_reachable itsl k2))
@@ -1448,9 +1468,8 @@ let lemma_proving_ancestor_greatest_depth (itsl: TL.eac_log) (k:key{k <> Root}) 
     else
       lemma_desc_depth_monotonic k' k2
   )
-  else lemma_first_root_reachable_ancestor_greatest_depth itsl k k2
+  else lemma_first_root_reachable_ancestor_greatest_depth pf k k2
   
-
 (* after the first add the proving ancestor always points to self *)
 let lemma_proving_ancestor_points_to_self (itsl: TL.eac_log) (k:key{k <> Root}):
   Lemma (requires not (is_eac_state_init itsl k))
@@ -1515,13 +1534,263 @@ let lemma_proving_ancestor_initial (itsl: TL.eac_log) (k:key{k <> Root}):
     (* nothing to prove if k is not a descendant of k2 *)
     else ()
 
+let proving_ancestor_has_hash (itsl: TL.eac_log) (k:key{k <> Root}): bool = 
+  not (is_eac_state_evicted_merkle itsl k) || 
+  mv_pointed_hash (eac_merkle_value itsl (proving_ancestor itsl k))
+                                         (desc_dir k (proving_ancestor itsl k)) =
+  hashfn (eac_value itsl k)
+
+let is_memory_op (e:vlog_entry): bool = 
+  match e with
+  | Get _ _ -> true
+  | Put _ _ -> true
+  | _ -> false
+
+let lemma_eac_value_root_unchanged (itsl: TL.eac_log {I.length itsl > 0}):
+  Lemma (requires (let n = I.length itsl in
+                   let e = I.index itsl (n - 1) in
+                   is_memory_op e))
+        (ensures (let n = I.length itsl in
+                  let itsl' = I.prefix itsl (n - 1) in
+                  eac_value itsl Root = eac_value itsl' Root)) = 
+  let n = I.length itsl in
+  let tid = TL.thread_id_of itsl (n - 1) in
+  let itsl' = I.prefix itsl (n - 1) in
+  lemma_fullprefix_equal itsl;
+  lemma_root_in_store0 itsl;
+  lemma_root_in_store0 itsl';
+  lemma_eac_value_is_stored_value itsl Root 0;
+  lemma_eac_value_is_stored_value itsl' Root 0;
+
+  if tid = 0 then 
+    lemma_verifier_thread_state_extend itsl (n - 1)  
+  else 
+    lemma_verifier_thread_state_extend2 itsl (n - 1) 0
+  
+let lemma_eac_value_unchanged (itsl: TL.eac_log {I.length itsl > 0}) (k: key):
+  Lemma (requires (let n = I.length itsl in
+                   let e = I.index itsl (n - 1) in
+                   is_memory_op e /\
+                   k <> V.key_of e))
+        (ensures (let n = I.length itsl in
+                  let itsl' = I.prefix itsl (n - 1) in
+                  eac_value itsl k = eac_value itsl' k)) = 
+ if k = Root then lemma_eac_value_root_unchanged itsl
+ else
+ let n = I.length itsl in
+ let e = I.index itsl (n - 1) in
+ let es = eac_state_of_key itsl k in
+ let itsl' = I.prefix itsl (n - 1) in
+ let tid = TL.thread_id_of itsl (n - 1) in
+
+ lemma_fullprefix_equal itsl;
+ lemma_eac_state_same itsl (n- 1) k;
+ lemma_eac_state_of_key_valid itsl k;
+ // assert(es = eac_state_of_key itsl' k);
+
+ match es with
+ | EACInit -> 
+   lemma_eac_value_init itsl k;
+   lemma_eac_value_init itsl' k
+
+ | EACInStore _ _ ->
+   let tidk = TL.stored_tid itsl k in
+   if tidk = tid then (
+     lemma_verifier_thread_state_extend itsl (n - 1);
+     lemma_eac_value_is_stored_value itsl k tidk;
+     lemma_eac_value_is_stored_value itsl' k tidk
+   )
+   else (
+     lemma_verifier_thread_state_extend2 itsl (n - 1) tidk;
+     lemma_eac_value_is_stored_value itsl k tidk;
+     lemma_eac_value_is_stored_value itsl' k tidk
+   )
+
+ | EACEvictedBlum _ _ _
+ | EACEvictedMerkle _ ->
+   lemma_eac_state_transition itsl (n - 1);
+   lemma_eac_state_same itsl (n - 1) k; 
+   lemma_eac_value_is_evicted_value itsl k;
+   lemma_eac_value_is_evicted_value itsl' k   
+
+let lemma_proving_ancestor_has_hash_extend_memop (itsl: TL.eac_log {I.length itsl > 0}) (k: key{k <> Root}):
+  Lemma (requires (let n = I.length itsl in
+                   let e = I.index itsl (n - 1) in
+                   let itsl' = I.prefix itsl (n - 1) in
+                   proving_ancestor_has_hash itsl' k /\
+                   (Get? e \/ Put? e)))
+        (ensures (proving_ancestor_has_hash itsl k)) = 
+  let n = I.length itsl in
+  let e = I.index itsl (n - 1) in
+  
+  let itsl' = I.prefix itsl (n - 1) in
+  let es' = TL.eac_state_of_key itsl' k in
+  
+  if not (is_eac_state_evicted_merkle itsl k) then ()
+  else (
+    lemma_fullprefix_equal itsl;
+    lemma_eac_state_transition itsl (n - 1);
+    lemma_eac_state_of_key_valid itsl' k;    
+    
+    lemma_eac_value_unchanged itsl k;
+    // assert(eac_value itsl k = eac_value itsl' k);
+    
+    lemma_ptrfn_unchanged itsl;
+    // assert(feq_ptrfn (eac_ptrfn itsl) (eac_ptrfn itsl'));
+
+    (* proving ancestor is unchanged when processing e *)
+    let pk = proving_ancestor itsl k in
+    lemma_feq_proving_ancestor (eac_ptrfn itsl) (eac_ptrfn itsl') k;    
+    // assert(pk = proving_ancestor itsl' k);
+
+    
+    lemma_eac_value_unchanged itsl pk;
+    // assert(eac_value itsl pk = eac_value itsl' pk);
+
+    lemma_eac_state_same itsl (n - 1) k
+  )
+
+let lemma_evict_ancestor_is_proving (itsl: TL.eac_log {I.length itsl > 0}):
+  Lemma (requires (let n = I.length itsl in
+                   let e = I.index itsl (n - 1) in
+                   EvictM? e))
+        (ensures (let n = I.length itsl in
+                  let e = I.index itsl (n - 1) in
+                  let k = EvictM?.k e in
+                  let k' = EvictM?.k' e in
+                  let itsl' = I.prefix itsl (n - 1) in
+                  k <> Root /\
+                  k' = proving_ancestor itsl' k)) = 
+  let n = I.length itsl in                      
+  let e = I.index itsl (n - 1) in
+  let tid = TL.thread_id_of itsl (n - 1) in
+  let itsl' = I.prefix itsl (n - 1) in
+  let pf' = eac_ptrfn itsl' in
+  match e with
+  | EvictM k k' ->
+    lemma_fullprefix_equal itsl;
+    lemma_verifier_thread_state_extend itsl (n - 1);
+
+    (* ptrfn of itsl and itsl' are identical *)
+    lemma_ptrfn_unchanged itsl;
+    // assert(feq_ptrfn (eac_ptrfn itsl) (eac_ptrfn itsl'));
+
+    lemma_eac_value_is_stored_value itsl' k' tid;
+    // assert(points_to pf' k k');
+
+    lemma_instore_implies_eac_state_instore itsl' k tid;
+    lemma_not_init_equiv_root_reachable itsl' k;
+    
+    let lemma_root_reachable_k' ():
+      Lemma (BP.root_reachable pf' k') = 
+      if k' = Root then
+        lemma_reachable_reflexive pf' Root
+      else (
+        lemma_instore_implies_eac_state_instore itsl' k' tid;
+        lemma_not_init_equiv_root_reachable itsl' k'
+      )
+    in
+    lemma_root_reachable_k'();
+    lemma_points_to_is_prev pf' k Root k' 
+
+let lemma_proving_ancestor_has_hash_extend_evictm (itsl: TL.eac_log {I.length itsl > 0}) (k: key{k <> Root}):
+  Lemma (requires (let n = I.length itsl in
+                   let e = I.index itsl (n - 1) in
+                   let itsl' = I.prefix itsl (n - 1) in
+                   proving_ancestor_has_hash itsl' k /\
+                   EvictM? e))
+        (ensures (proving_ancestor_has_hash itsl k)) = 
+  let n = I.length itsl in
+  let e = I.index itsl (n - 1) in
+  let tid = TL.thread_id_of itsl (n - 1) in
+  let vs = TL.thread_state itsl tid in
+  let itsl' = I.prefix itsl (n - 1) in
+  let es' = TL.eac_state_of_key itsl' k in
+  let vs' = TL.thread_state itsl' tid in
+  let st' = TL.thread_store itsl' tid in
+
+  if not (is_eac_state_evicted_merkle itsl k) then ()
+  else (
+
+    match e with
+    | EvictM k1 k2 ->
+
+      lemma_fullprefix_equal itsl;
+      lemma_verifier_thread_state_extend itsl (n - 1);
+
+      if k1 = k then (
+        // assert(V.store_contains st' k);
+        lemma_eac_value_is_stored_value itsl' k tid;
+        // assert(eac_value itsl' k = V.stored_value st' k);
+
+        lemma_eac_state_transition itsl (n - 1);
+        lemma_instore_implies_eac_state_instore itsl' k tid;
+        lemma_ext_evict_val_is_stored_val itsl (n - 1);
+        lemma_eac_value_is_evicted_value itsl k;
+        // assert(eac_value itsl k = eac_value itsl' k);
+
+        lemma_ptrfn_unchanged itsl;
+        // assert(feq_ptrfn (eac_ptrfn itsl) (eac_ptrfn itsl'));
+
+        (* proving ancestor is unchanged when processing e *)
+        let pk = proving_ancestor itsl k in
+        lemma_feq_proving_ancestor (eac_ptrfn itsl) (eac_ptrfn itsl') k;
+
+        lemma_evict_ancestor_is_proving itsl;
+        // assert(pk = k2);
+
+        lemma_eac_value_is_stored_value itsl pk tid
+      )
+      else if k2 = k then 
+        lemma_instore_implies_eac_state_instore itsl k tid
+      else (
+        lemma_eac_state_same itsl (n - 1) k;
+        lemma_eac_value_is_evicted_value itsl k;
+        lemma_eac_value_is_evicted_value itsl' k;
+        assert(eac_value itsl k = eac_value itsl' k);
+
+        lemma_ptrfn_unchanged itsl;
+        let pk = proving_ancestor itsl k in
+        lemma_feq_proving_ancestor (eac_ptrfn itsl) (eac_ptrfn itsl') k;
+
+        admit()
+      )
+  )
+
+
+(* when evicted as merkle the proving ancestor contains our hash *)
+let rec lemma_proving_ancestor_has_hash_aux (itsl: TL.eac_log) (k:key{k<> Root}):
+  Lemma (requires True)
+        (ensures (proving_ancestor_has_hash itsl k))
+        (decreases (I.length itsl)) =
+  let n = I.length itsl in
+  if n = 0 then
+    lemma_init_state_empty itsl k
+  else if not (is_eac_state_evicted_merkle itsl k) then ()
+  else (
+    let e = I.index itsl (n - 1) in
+    let itsl' = I.prefix itsl (n - 1) in
+
+    (* induction *)
+    lemma_proving_ancestor_has_hash_aux itsl' k;
+
+    match e with
+    | Get _ _ 
+    | Put _ _ -> 
+      lemma_proving_ancestor_has_hash_extend_memop itsl k
+    | EvictM _ _ ->
+      lemma_proving_ancestor_has_hash_extend_evictm itsl k
+    | _ ->
+
+    admit()
+  )
+
 (* when evicted as merkle the proving ancestor contains our hash *)
 let lemma_proving_ancestor_has_hash (itsl: TL.eac_log) (k:key{k<> Root}):
   Lemma (requires (is_eac_state_evicted_merkle itsl k))
         (ensures (mv_pointed_hash (eac_merkle_value itsl (proving_ancestor itsl k))
                                   (desc_dir k (proving_ancestor itsl k)) =
-                  hashfn (eac_value itsl k))) =
-  admit()
+                  hashfn (eac_value itsl k))) = lemma_proving_ancestor_has_hash_aux itsl k
 
 (* when evicted as blum the proving ancestor contains a bit indicating the eviction *)
 let lemma_proving_ancestor_blum_bit (itsl: TL.eac_log) (k:key{k <> Root}):
